progress?

dfy/cnf.dfy
@@ -20,11 +20,128 @@ ghost function cnf_equivalent(cnf: CNF, other: CNF) : (eq: bool)
         cnf_eval(cnf,vs) == cnf_eval(other, vs)
 }
 
+predicate cnf_has_tautologies(cnf: CNF)
+{
+    exists c :: c in cnf && clause_is_tautology(c)
+}
 
 function cnf_remove_tautologies(cnf: CNF) : (out: CNF)
     ensures cnf_equivalent(cnf, out)
+    ensures !cnf_has_tautologies(out)
 {
     set c | c in cnf && !clause_is_tautology(c)
 }
+
+
+function clause_max_litvar(c: Clause) : (out: ClauseLit)
+    requires |c| > 0
+{
+    if |c| == 1 then
+        Util.extract_only_from_set(c)
+    else
+        var lambda := (l: ClauseLit) => l.number();
+        SAT.NumbersBijection(c, lambda);
+        Util.extract_max_from_set(c, lambda)
+}
+
+// function clause_gt(c1: Clause, c2: Clause) : (out: bool)
+//     requires c1 != c2
+// {
+//     if |c1| > |c2| then
+//         true
+//     else if |c1| < |c2| then
+//         false
+//     else
+//         assert |c1| == |c2|;
+
+// }
+
+// function max_clause(cs: set<Clause>) : (out: Clause)
+//     requires |cs| > 0
+// {
+//     var c :| c in cs && forall cc :: cc in cs && cc != c ==>  c >= cc;
+//     c
+// }
+
+// function cnf_find_resolution_with_var(cnf: CNF, v: Variable) : (out: set<Clause>)
+//     requires !cnf_has_tautologies(cnf)
+//     // ensures (exists l1, l2, c1, c2 ::
+//     //     v in cnf_vars(cnf) &&
+//     //     c1 in cnf && c2 in cnf && c1 != c2 &&
+//     //     l1 in c1 && NotInverted(v) == l1 &&
+//     //     l2 in c2 && Inverted(v) == l2) <==> |out| == 2
+//     ensures |out| == 0 || |out| == 2
+// {
+//     var where_inverted := set c | c in cnf && Inverted(v) in c;
+//     var where_not_inverted := set c | c in cnf && NotInverted(v) in c;
+//     assert |where_inverted * where_not_inverted| == 0;
+//     if |where_inverted| > 0 && |where_not_inverted| > 0 then
+//         var c1 :| c1 in where_inverted && forall c :: c in where_inverted && c != c1 && c1 > c;
+//         var c2 :| c2 in where_not_inverted;
+//         {c1, c2}
+//     else
+//         {}
+// }
+
+// function cnf_has_resolution(cnf: CNF) : (out: bool)
+//     ensures out == (exists v :: v in cnf_vars(cnf) && cnf_has_resolution_with_var(cnf, v))
+// {
+//     exists v :: v in cnf_vars(cnf) && cnf_has_resolution_with_var(cnf, v)
+// }
+
+// function cnf_has_resolution_with_var(cnf: CNF, v: Variable) : (out: bool)
+//     ensures out == (exists l1, l2, c1, c2 ::
+//         v in cnf_vars(cnf) &&
+//         c1 in cnf && c2 in cnf && c1 != c2 &&
+//         l1 in c1 && NotInverted(v) == l1 &&
+//         l2 in c2 && Inverted(v) == l2)
+// {
+//     exists l1, l2, c1, c2 ::
+//         v in cnf_vars(cnf) &&
+//         c1 in cnf && c2 in cnf && c1 != c2 &&
+//         l1 in c1 && NotInverted(v) == l1 &&
+//         l2 in c2 && Inverted(v) == l2
+// }
+
+// ghost function cnf_some_resolution_var(cnf: CNF) : (v: Variable)
+//     requires cnf_has_resolution(cnf)
+//     ensures exists l1, l2, c1, c2 ::
+//         c1 in cnf && c2 in cnf && c1 != c2 &&
+//         l1 in c1 && NotInverted(v) == l1 &&
+//         l2 in c2 && Inverted(v) == l2
+// {
+//     assert exists v :: v in cnf_vars(cnf) && cnf_has_resolution_with_var(cnf, v);
+//     var v :| v in cnf_vars(cnf) && cnf_has_resolution_with_var(cnf, v);
+//     v
+// }
+
+// function cnf_clauses_with_var(cnf: CNF, ls: set<ClauseLit>) : (out: set<Clause>)
+//     ensures forall c :: c in cnf && (exists l :: l in ls && l in c) <==> c in out
+// {
+//     set c | c in cnf && (exists l :: l in ls && l in c)
+// }
+
+// function cnf_resolution(cnf: CNF) : (out: CNF)
+//     requires !cnf_has_tautologies(cnf)
+//     requires cnf_has_resolution(cnf)
+//     ensures cnf_equivalent(cnf, out)
+// {
+//     var v := cnf_some_resolution_var(cnf);
+//     assert exists l1, l2, c1, c2 ::
+//         c1 in cnf && c2 in cnf && c1 != c2 &&
+//         l1 in c1 && NotInverted(v) == l1 &&
+//         l2 in c2 && Inverted(v) == l2;
+//     assert exists c :: c in cnf && NotInverted(v) in c;
+
+//     var where_not_inverted: set<Clause> := set c | c in cnf && NotInverted(v) in c;
+//     assert |where_not_inverted| > 0;
+//     // var where_inverted: set<Clause> := set c | c in cnf && Inverted(v) in c;
+//     // assert |where_inverted| > 0;
+
+//     // var c1 :| c1 in not_inverted[v];
+//     // var c2 :| c2 in inverted[v];
+
+//     cnf
+// }
 
 }
